backend/Debugvarproof.v
@@ -297,14 +297,14 @@ Let tge := Senv.globalenv tprog se.
 
 Lemma symbols_preserved:
   forall (s: ident), Genv.find_symbol tge s = Genv.find_symbol ge s.
-Proof. apply Senv.find_symbol_match. Qed.
+Proof. apply Senv.find_symbol_match_id. Qed.
 
 Lemma functions_translated:
   forall (v: val) (f: fundef),
   Genv.find_funct ge v = Some f ->
   exists tf,
   Genv.find_funct tge v = Some tf /\ transf_fundef f = OK tf.
-Proof. exact (Senv.find_funct_transf_partial TRANSF). Qed.
+Proof. exact (Senv.find_funct_transf_partial_id TRANSF). Qed.
 
 Lemma sig_preserved:
   forall f tf,
@@ -543,7 +543,7 @@ Theorem transf_program_correct prog tprog:
   match_prog prog tprog ->
   open_fsim cc_id cc_id (semantics prog) (semantics tprog).
 Proof.
-  intros MATCH [ ] se _ q _ _ [ ] [ ].
+  intros MATCH [ ] se _ q _ _ _ [ ] [ ].
   eapply forward_simulation_plus; simpl.
   - eauto using transf_initial_states.
   - eauto using transf_final_states.
